Added refinement of IMP_Minus_State_To_IMP_Minus_Minus_partial_tail_aux3

Cook_Levin/IMP-_To_SAS+/IMP-_To_IMP--/IMP_Minus_To_IMP_Minus_Minus_State_Translations_IMP.thy
@@ -6113,7 +6113,7 @@ lemma IMP_Minus_State_To_IMP_Minus_Minus_partial_tail_aux2_IMP_Minus_correct:
     IMP_Minus_State_To_IMP_Minus_Minus_partial_tail_aux2_IMP_Minus_correct_effects
   by (meson set_mono_prefix)
 
-(* ---------------------------------------------------------------------------------------------- *)
+
 
 fun IMP_Minus_State_To_IMP_Minus_Minus_partial_tail_aux3 :: "nat \<Rightarrow> nat \<Rightarrow> nat \<Rightarrow> nat \<Rightarrow> nat \<Rightarrow> nat" where
   "IMP_Minus_State_To_IMP_Minus_Minus_partial_tail_aux3 n v po vo ko =
@@ -6122,6 +6122,471 @@ fun IMP_Minus_State_To_IMP_Minus_Minus_partial_tail_aux3 :: "nat \<Rightarrow> n
           then Suc 0
           else 0
      else IMP_Minus_State_To_IMP_Minus_Minus_partial_tail_aux2 n v po vo ko)"
+
+record IMP_Minus_State_To_IMP_Minus_Minus_partial_tail_aux3_state =
+  IMP_Minus_State_To_IMP_Minus_Minus_partial_tail_aux3_n::nat
+  IMP_Minus_State_To_IMP_Minus_Minus_partial_tail_aux3_v::nat
+  IMP_Minus_State_To_IMP_Minus_Minus_partial_tail_aux3_po::nat
+  IMP_Minus_State_To_IMP_Minus_Minus_partial_tail_aux3_vo::nat
+  IMP_Minus_State_To_IMP_Minus_Minus_partial_tail_aux3_ko::nat
+  IMP_Minus_State_To_IMP_Minus_Minus_partial_tail_aux3_ret::nat
+
+abbreviation "IMP_Minus_State_To_IMP_Minus_Minus_partial_tail_aux3_prefix \<equiv> ''IMP_Minus_State_To_IMP_Minus_Minus_partial_tail_aux3.''"
+abbreviation "IMP_Minus_State_To_IMP_Minus_Minus_partial_tail_aux3_n_str \<equiv> ''n''"
+abbreviation "IMP_Minus_State_To_IMP_Minus_Minus_partial_tail_aux3_v_str \<equiv> ''v''"
+abbreviation "IMP_Minus_State_To_IMP_Minus_Minus_partial_tail_aux3_po_str \<equiv> ''po''"
+abbreviation "IMP_Minus_State_To_IMP_Minus_Minus_partial_tail_aux3_vo_str \<equiv> ''vo''"
+abbreviation "IMP_Minus_State_To_IMP_Minus_Minus_partial_tail_aux3_ko_str \<equiv> ''ko''"
+abbreviation "IMP_Minus_State_To_IMP_Minus_Minus_partial_tail_aux3_ret_str \<equiv> ''ret''"
+
+definition "IMP_Minus_State_To_IMP_Minus_Minus_partial_tail_aux3_state_upd s \<equiv>
+  (let
+      EQUAL_neq_zero_a' = IMP_Minus_State_To_IMP_Minus_Minus_partial_tail_aux3_vo s;
+      EQUAL_neq_zero_b' = a_encode_char_as_nat;
+      EQUAL_neq_zero_ret' = 0;
+      EQUAL_neq_zero_state = \<lparr>EQUAL_neq_zero_a = EQUAL_neq_zero_a',
+                              EQUAL_neq_zero_b = EQUAL_neq_zero_b',
+                              EQUAL_neq_zero_ret = EQUAL_neq_zero_ret'\<rparr>;
+      EQUAL_neq_zero_ret_state = EQUAL_neq_zero_imp EQUAL_neq_zero_state;
+      AND_neq_zero_a' = IMP_Minus_State_To_IMP_Minus_Minus_partial_tail_aux3_po s;
+      AND_neq_zero_b' = EQUAL_neq_zero_ret EQUAL_neq_zero_ret_state;
+      AND_neq_zero_ret' = 0;
+      AND_neq_zero_state = \<lparr>AND_neq_zero_a = AND_neq_zero_a',
+                            AND_neq_zero_b = AND_neq_zero_b',
+                            AND_neq_zero_ret = AND_neq_zero_ret'\<rparr>;
+      AND_neq_zero_ret_state = AND_neq_zero_imp AND_neq_zero_state;
+      AND_neq_zero_result = AND_neq_zero_ret AND_neq_zero_ret_state
+  in
+  (if AND_neq_zero_result \<noteq> 0 then
+  (let 
+      LESS_neq_zero_a' = IMP_Minus_State_To_IMP_Minus_Minus_partial_tail_aux3_ko s;
+      LESS_neq_zero_b' = IMP_Minus_State_To_IMP_Minus_Minus_partial_tail_aux3_n s;
+      LESS_neq_zero_ret' = 0;
+      LESS_neq_zero_state = \<lparr>LESS_neq_zero_a = LESS_neq_zero_a',
+                             LESS_neq_zero_b = LESS_neq_zero_b',
+                             LESS_neq_zero_ret = LESS_neq_zero_ret'\<rparr>;
+      LESS_neq_zero_ret_state = LESS_neq_zero_imp LESS_neq_zero_state;
+      LESS_neq_zero_result = LESS_neq_zero_ret LESS_neq_zero_ret_state
+  in   
+  (if LESS_neq_zero_result \<noteq> 0 then
+  (let 
+      IMP_Minus_State_To_IMP_Minus_Minus_partial_tail_aux3_ret' = 1;
+      ret = \<lparr>IMP_Minus_State_To_IMP_Minus_Minus_partial_tail_aux3_n = IMP_Minus_State_To_IMP_Minus_Minus_partial_tail_aux3_n s,
+             IMP_Minus_State_To_IMP_Minus_Minus_partial_tail_aux3_v = IMP_Minus_State_To_IMP_Minus_Minus_partial_tail_aux3_v s,
+             IMP_Minus_State_To_IMP_Minus_Minus_partial_tail_aux3_po = IMP_Minus_State_To_IMP_Minus_Minus_partial_tail_aux3_po s,
+             IMP_Minus_State_To_IMP_Minus_Minus_partial_tail_aux3_vo = IMP_Minus_State_To_IMP_Minus_Minus_partial_tail_aux3_vo s,
+             IMP_Minus_State_To_IMP_Minus_Minus_partial_tail_aux3_ko = IMP_Minus_State_To_IMP_Minus_Minus_partial_tail_aux3_ko s,
+             IMP_Minus_State_To_IMP_Minus_Minus_partial_tail_aux3_ret = IMP_Minus_State_To_IMP_Minus_Minus_partial_tail_aux3_ret'\<rparr>
+  in
+      ret
+  )
+  else
+  (let 
+      IMP_Minus_State_To_IMP_Minus_Minus_partial_tail_aux3_ret' = 0;
+      ret = \<lparr>IMP_Minus_State_To_IMP_Minus_Minus_partial_tail_aux3_n = IMP_Minus_State_To_IMP_Minus_Minus_partial_tail_aux3_n s,
+             IMP_Minus_State_To_IMP_Minus_Minus_partial_tail_aux3_v = IMP_Minus_State_To_IMP_Minus_Minus_partial_tail_aux3_v s,
+             IMP_Minus_State_To_IMP_Minus_Minus_partial_tail_aux3_po = IMP_Minus_State_To_IMP_Minus_Minus_partial_tail_aux3_po s,
+             IMP_Minus_State_To_IMP_Minus_Minus_partial_tail_aux3_vo = IMP_Minus_State_To_IMP_Minus_Minus_partial_tail_aux3_vo s,
+             IMP_Minus_State_To_IMP_Minus_Minus_partial_tail_aux3_ko = IMP_Minus_State_To_IMP_Minus_Minus_partial_tail_aux3_ko s,
+             IMP_Minus_State_To_IMP_Minus_Minus_partial_tail_aux3_ret = IMP_Minus_State_To_IMP_Minus_Minus_partial_tail_aux3_ret'\<rparr>
+  in
+      ret
+  )))
+  else
+  (let 
+      IMP_Minus_State_To_IMP_Minus_Minus_partial_tail_aux2_n' = IMP_Minus_State_To_IMP_Minus_Minus_partial_tail_aux3_n s;
+      IMP_Minus_State_To_IMP_Minus_Minus_partial_tail_aux2_v' = IMP_Minus_State_To_IMP_Minus_Minus_partial_tail_aux3_v s;
+      IMP_Minus_State_To_IMP_Minus_Minus_partial_tail_aux2_po' = IMP_Minus_State_To_IMP_Minus_Minus_partial_tail_aux3_po s;
+      IMP_Minus_State_To_IMP_Minus_Minus_partial_tail_aux2_vo' = IMP_Minus_State_To_IMP_Minus_Minus_partial_tail_aux3_vo s;
+      IMP_Minus_State_To_IMP_Minus_Minus_partial_tail_aux2_ko' = IMP_Minus_State_To_IMP_Minus_Minus_partial_tail_aux3_ko s;
+      IMP_Minus_State_To_IMP_Minus_Minus_partial_tail_aux2_ret' = 0;
+      IMP_Minus_State_To_IMP_Minus_Minus_partial_tail_aux2_state =
+        \<lparr>IMP_Minus_State_To_IMP_Minus_Minus_partial_tail_aux2_n = IMP_Minus_State_To_IMP_Minus_Minus_partial_tail_aux2_n',
+         IMP_Minus_State_To_IMP_Minus_Minus_partial_tail_aux2_v = IMP_Minus_State_To_IMP_Minus_Minus_partial_tail_aux2_v',
+         IMP_Minus_State_To_IMP_Minus_Minus_partial_tail_aux2_po = IMP_Minus_State_To_IMP_Minus_Minus_partial_tail_aux2_po',
+         IMP_Minus_State_To_IMP_Minus_Minus_partial_tail_aux2_vo = IMP_Minus_State_To_IMP_Minus_Minus_partial_tail_aux2_vo',
+         IMP_Minus_State_To_IMP_Minus_Minus_partial_tail_aux2_ko = IMP_Minus_State_To_IMP_Minus_Minus_partial_tail_aux2_ko',
+         IMP_Minus_State_To_IMP_Minus_Minus_partial_tail_aux2_ret = IMP_Minus_State_To_IMP_Minus_Minus_partial_tail_aux2_ret'\<rparr>;
+      IMP_Minus_State_To_IMP_Minus_Minus_partial_tail_aux2_ret_state =
+        IMP_Minus_State_To_IMP_Minus_Minus_partial_tail_aux2_imp IMP_Minus_State_To_IMP_Minus_Minus_partial_tail_aux2_state;
+      IMP_Minus_State_To_IMP_Minus_Minus_partial_tail_aux3_ret' = 
+        IMP_Minus_State_To_IMP_Minus_Minus_partial_tail_aux2_ret IMP_Minus_State_To_IMP_Minus_Minus_partial_tail_aux2_ret_state;
+      ret = \<lparr>IMP_Minus_State_To_IMP_Minus_Minus_partial_tail_aux3_n = IMP_Minus_State_To_IMP_Minus_Minus_partial_tail_aux3_n s,
+             IMP_Minus_State_To_IMP_Minus_Minus_partial_tail_aux3_v = IMP_Minus_State_To_IMP_Minus_Minus_partial_tail_aux3_v s,
+             IMP_Minus_State_To_IMP_Minus_Minus_partial_tail_aux3_po = IMP_Minus_State_To_IMP_Minus_Minus_partial_tail_aux3_po s,
+             IMP_Minus_State_To_IMP_Minus_Minus_partial_tail_aux3_vo = IMP_Minus_State_To_IMP_Minus_Minus_partial_tail_aux3_vo s,
+             IMP_Minus_State_To_IMP_Minus_Minus_partial_tail_aux3_ko = IMP_Minus_State_To_IMP_Minus_Minus_partial_tail_aux3_ko s,
+             IMP_Minus_State_To_IMP_Minus_Minus_partial_tail_aux3_ret = IMP_Minus_State_To_IMP_Minus_Minus_partial_tail_aux3_ret'\<rparr>
+  in
+      ret
+  )))"
+
+function IMP_Minus_State_To_IMP_Minus_Minus_partial_tail_aux3_imp ::
+  "IMP_Minus_State_To_IMP_Minus_Minus_partial_tail_aux3_state \<Rightarrow> IMP_Minus_State_To_IMP_Minus_Minus_partial_tail_aux3_state" where
+  "IMP_Minus_State_To_IMP_Minus_Minus_partial_tail_aux3_imp s =
+  (let 
+      ret = IMP_Minus_State_To_IMP_Minus_Minus_partial_tail_aux3_state_upd s
+    in 
+      ret
+  )"
+  by simp+
+termination
+  by (relation "measure IMP_Minus_State_To_IMP_Minus_Minus_partial_tail_aux3_n") simp
+
+declare IMP_Minus_State_To_IMP_Minus_Minus_partial_tail_aux3_imp.simps [simp del]
+
+lemma IMP_Minus_State_To_IMP_Minus_Minus_partial_tail_aux3_imp_correct[let_function_correctness]:
+  "IMP_Minus_State_To_IMP_Minus_Minus_partial_tail_aux3_ret (IMP_Minus_State_To_IMP_Minus_Minus_partial_tail_aux3_imp s) =
+    IMP_Minus_State_To_IMP_Minus_Minus_partial_tail_aux3
+      (IMP_Minus_State_To_IMP_Minus_Minus_partial_tail_aux3_n s) (IMP_Minus_State_To_IMP_Minus_Minus_partial_tail_aux3_v s)
+      (IMP_Minus_State_To_IMP_Minus_Minus_partial_tail_aux3_po s) (IMP_Minus_State_To_IMP_Minus_Minus_partial_tail_aux3_vo s)
+      (IMP_Minus_State_To_IMP_Minus_Minus_partial_tail_aux3_ko s)"
+  apply (simp only: IMP_Minus_State_To_IMP_Minus_Minus_partial_tail_aux3_imp.simps Let_def 
+  IMP_Minus_State_To_IMP_Minus_Minus_partial_tail_aux3_state_upd_def EQUAL_neq_zero_imp_correct
+  AND_neq_zero_imp_correct LESS_neq_zero_imp_correct IMP_Minus_State_To_IMP_Minus_Minus_partial_tail_aux2_imp_correct
+  a_encode_char_val IMP_Minus_State_To_IMP_Minus_Minus_partial_tail_aux3.simps)
+  by simp
+
+function IMP_Minus_State_To_IMP_Minus_Minus_partial_tail_aux3_imp_time ::
+  "nat \<Rightarrow> IMP_Minus_State_To_IMP_Minus_Minus_partial_tail_aux3_state \<Rightarrow> nat" where
+  "IMP_Minus_State_To_IMP_Minus_Minus_partial_tail_aux3_imp_time t s =
+  (let
+      EQUAL_neq_zero_a' = IMP_Minus_State_To_IMP_Minus_Minus_partial_tail_aux3_vo s;
+      t = t + 2;
+      EQUAL_neq_zero_b' = a_encode_char_as_nat;
+      t = t + 2;
+      EQUAL_neq_zero_ret' = 0;
+      t = t + 2;
+      EQUAL_neq_zero_state = \<lparr>EQUAL_neq_zero_a = EQUAL_neq_zero_a',
+                              EQUAL_neq_zero_b = EQUAL_neq_zero_b',
+                              EQUAL_neq_zero_ret = EQUAL_neq_zero_ret'\<rparr>;
+      EQUAL_neq_zero_ret_state = EQUAL_neq_zero_imp EQUAL_neq_zero_state;
+      t = t + EQUAL_neq_zero_imp_time 0 EQUAL_neq_zero_state;
+      AND_neq_zero_a' = IMP_Minus_State_To_IMP_Minus_Minus_partial_tail_aux3_po s;
+      t = t + 2;
+      AND_neq_zero_b' = EQUAL_neq_zero_ret EQUAL_neq_zero_ret_state;
+      t = t + 2;
+      AND_neq_zero_ret' = 0;
+      t = t + 2;
+      AND_neq_zero_state = \<lparr>AND_neq_zero_a = AND_neq_zero_a',
+                            AND_neq_zero_b = AND_neq_zero_b',
+                            AND_neq_zero_ret = AND_neq_zero_ret'\<rparr>;
+      AND_neq_zero_ret_state = AND_neq_zero_imp AND_neq_zero_state;
+      t = t + AND_neq_zero_imp_time 0 AND_neq_zero_state;
+      AND_neq_zero_result = AND_neq_zero_ret AND_neq_zero_ret_state;
+      t = t + 2
+  in
+  (if AND_neq_zero_result \<noteq> 0 then
+  (let 
+      t = t + 1;
+      LESS_neq_zero_a' = IMP_Minus_State_To_IMP_Minus_Minus_partial_tail_aux3_ko s;
+      t = t + 2;
+      LESS_neq_zero_b' = IMP_Minus_State_To_IMP_Minus_Minus_partial_tail_aux3_n s;
+      t = t + 2;
+      LESS_neq_zero_ret' = 0;
+      t = t + 2;
+      LESS_neq_zero_state = \<lparr>LESS_neq_zero_a = LESS_neq_zero_a',
+                             LESS_neq_zero_b = LESS_neq_zero_b',
+                             LESS_neq_zero_ret = LESS_neq_zero_ret'\<rparr>;
+      LESS_neq_zero_ret_state = LESS_neq_zero_imp LESS_neq_zero_state;
+      t = t + LESS_neq_zero_imp_time 0 LESS_neq_zero_state;
+      LESS_neq_zero_result = LESS_neq_zero_ret LESS_neq_zero_ret_state;
+      t = t + 2
+  in   
+  (if LESS_neq_zero_result \<noteq> 0 then
+  (let 
+      t = t + 1;
+      IMP_Minus_State_To_IMP_Minus_Minus_partial_tail_aux3_ret' = 1;
+      t = t + 2;
+      ret = \<lparr>IMP_Minus_State_To_IMP_Minus_Minus_partial_tail_aux3_n = IMP_Minus_State_To_IMP_Minus_Minus_partial_tail_aux3_n s,
+             IMP_Minus_State_To_IMP_Minus_Minus_partial_tail_aux3_v = IMP_Minus_State_To_IMP_Minus_Minus_partial_tail_aux3_v s,
+             IMP_Minus_State_To_IMP_Minus_Minus_partial_tail_aux3_po = IMP_Minus_State_To_IMP_Minus_Minus_partial_tail_aux3_po s,
+             IMP_Minus_State_To_IMP_Minus_Minus_partial_tail_aux3_vo = IMP_Minus_State_To_IMP_Minus_Minus_partial_tail_aux3_vo s,
+             IMP_Minus_State_To_IMP_Minus_Minus_partial_tail_aux3_ko = IMP_Minus_State_To_IMP_Minus_Minus_partial_tail_aux3_ko s,
+             IMP_Minus_State_To_IMP_Minus_Minus_partial_tail_aux3_ret = IMP_Minus_State_To_IMP_Minus_Minus_partial_tail_aux3_ret'\<rparr>
+  in
+      t
+  )
+  else
+  (let 
+      t = t + 1;
+      IMP_Minus_State_To_IMP_Minus_Minus_partial_tail_aux3_ret' = 0;
+      t = t + 2;
+      ret = \<lparr>IMP_Minus_State_To_IMP_Minus_Minus_partial_tail_aux3_n = IMP_Minus_State_To_IMP_Minus_Minus_partial_tail_aux3_n s,
+             IMP_Minus_State_To_IMP_Minus_Minus_partial_tail_aux3_v = IMP_Minus_State_To_IMP_Minus_Minus_partial_tail_aux3_v s,
+             IMP_Minus_State_To_IMP_Minus_Minus_partial_tail_aux3_po = IMP_Minus_State_To_IMP_Minus_Minus_partial_tail_aux3_po s,
+             IMP_Minus_State_To_IMP_Minus_Minus_partial_tail_aux3_vo = IMP_Minus_State_To_IMP_Minus_Minus_partial_tail_aux3_vo s,
+             IMP_Minus_State_To_IMP_Minus_Minus_partial_tail_aux3_ko = IMP_Minus_State_To_IMP_Minus_Minus_partial_tail_aux3_ko s,
+             IMP_Minus_State_To_IMP_Minus_Minus_partial_tail_aux3_ret = IMP_Minus_State_To_IMP_Minus_Minus_partial_tail_aux3_ret'\<rparr>
+  in
+      t
+  )))
+  else
+  (let 
+      t = t + 1;
+      IMP_Minus_State_To_IMP_Minus_Minus_partial_tail_aux2_n' = IMP_Minus_State_To_IMP_Minus_Minus_partial_tail_aux3_n s;
+      t = t + 2;
+      IMP_Minus_State_To_IMP_Minus_Minus_partial_tail_aux2_v' = IMP_Minus_State_To_IMP_Minus_Minus_partial_tail_aux3_v s;
+      t = t + 2;
+      IMP_Minus_State_To_IMP_Minus_Minus_partial_tail_aux2_po' = IMP_Minus_State_To_IMP_Minus_Minus_partial_tail_aux3_po s;
+      t = t + 2;
+      IMP_Minus_State_To_IMP_Minus_Minus_partial_tail_aux2_vo' = IMP_Minus_State_To_IMP_Minus_Minus_partial_tail_aux3_vo s;
+      t = t + 2;
+      IMP_Minus_State_To_IMP_Minus_Minus_partial_tail_aux2_ko' = IMP_Minus_State_To_IMP_Minus_Minus_partial_tail_aux3_ko s;
+      t = t + 2;
+      IMP_Minus_State_To_IMP_Minus_Minus_partial_tail_aux2_ret' = 0;
+      t = t + 2;
+      IMP_Minus_State_To_IMP_Minus_Minus_partial_tail_aux2_state =
+        \<lparr>IMP_Minus_State_To_IMP_Minus_Minus_partial_tail_aux2_n = IMP_Minus_State_To_IMP_Minus_Minus_partial_tail_aux2_n',
+         IMP_Minus_State_To_IMP_Minus_Minus_partial_tail_aux2_v = IMP_Minus_State_To_IMP_Minus_Minus_partial_tail_aux2_v',
+         IMP_Minus_State_To_IMP_Minus_Minus_partial_tail_aux2_po = IMP_Minus_State_To_IMP_Minus_Minus_partial_tail_aux2_po',
+         IMP_Minus_State_To_IMP_Minus_Minus_partial_tail_aux2_vo = IMP_Minus_State_To_IMP_Minus_Minus_partial_tail_aux2_vo',
+         IMP_Minus_State_To_IMP_Minus_Minus_partial_tail_aux2_ko = IMP_Minus_State_To_IMP_Minus_Minus_partial_tail_aux2_ko',
+         IMP_Minus_State_To_IMP_Minus_Minus_partial_tail_aux2_ret = IMP_Minus_State_To_IMP_Minus_Minus_partial_tail_aux2_ret'\<rparr>;
+      IMP_Minus_State_To_IMP_Minus_Minus_partial_tail_aux2_ret_state =
+        IMP_Minus_State_To_IMP_Minus_Minus_partial_tail_aux2_imp IMP_Minus_State_To_IMP_Minus_Minus_partial_tail_aux2_state;
+      t = t + IMP_Minus_State_To_IMP_Minus_Minus_partial_tail_aux2_imp_time 0 IMP_Minus_State_To_IMP_Minus_Minus_partial_tail_aux2_state;
+      IMP_Minus_State_To_IMP_Minus_Minus_partial_tail_aux3_ret' = 
+        IMP_Minus_State_To_IMP_Minus_Minus_partial_tail_aux2_ret IMP_Minus_State_To_IMP_Minus_Minus_partial_tail_aux2_ret_state;
+      t = t + 2;
+      ret = \<lparr>IMP_Minus_State_To_IMP_Minus_Minus_partial_tail_aux3_n = IMP_Minus_State_To_IMP_Minus_Minus_partial_tail_aux3_n s,
+             IMP_Minus_State_To_IMP_Minus_Minus_partial_tail_aux3_v = IMP_Minus_State_To_IMP_Minus_Minus_partial_tail_aux3_v s,
+             IMP_Minus_State_To_IMP_Minus_Minus_partial_tail_aux3_po = IMP_Minus_State_To_IMP_Minus_Minus_partial_tail_aux3_po s,
+             IMP_Minus_State_To_IMP_Minus_Minus_partial_tail_aux3_vo = IMP_Minus_State_To_IMP_Minus_Minus_partial_tail_aux3_vo s,
+             IMP_Minus_State_To_IMP_Minus_Minus_partial_tail_aux3_ko = IMP_Minus_State_To_IMP_Minus_Minus_partial_tail_aux3_ko s,
+             IMP_Minus_State_To_IMP_Minus_Minus_partial_tail_aux3_ret = IMP_Minus_State_To_IMP_Minus_Minus_partial_tail_aux3_ret'\<rparr>
+  in
+      t
+  )))"
+  by auto
+termination
+  by (relation "measure (IMP_Minus_State_To_IMP_Minus_Minus_partial_tail_aux3_n \<circ> snd)") simp
+
+declare IMP_Minus_State_To_IMP_Minus_Minus_partial_tail_aux3_imp_time.simps [simp del]
+
+lemma IMP_Minus_State_To_IMP_Minus_Minus_partial_tail_aux3_imp_time_acc:
+  "(IMP_Minus_State_To_IMP_Minus_Minus_partial_tail_aux3_imp_time (Suc t) s) = Suc (IMP_Minus_State_To_IMP_Minus_Minus_partial_tail_aux3_imp_time t s)"
+  by (induction t s rule: IMP_Minus_State_To_IMP_Minus_Minus_partial_tail_aux3_imp_time.induct)
+    ((subst (1 2) IMP_Minus_State_To_IMP_Minus_Minus_partial_tail_aux3_imp_time.simps);
+      (simp add: IMP_Minus_State_To_IMP_Minus_Minus_partial_tail_aux3_state_upd_def Let_def))            
+
+lemma IMP_Minus_State_To_IMP_Minus_Minus_partial_tail_aux3_imp_time_acc_2_aux:
+  "(IMP_Minus_State_To_IMP_Minus_Minus_partial_tail_aux3_imp_time t s) = t + (IMP_Minus_State_To_IMP_Minus_Minus_partial_tail_aux3_imp_time 0 s)"
+  by (induction t arbitrary: s) (simp add: IMP_Minus_State_To_IMP_Minus_Minus_partial_tail_aux3_imp_time_acc)+            
+
+lemma IMP_Minus_State_To_IMP_Minus_Minus_partial_tail_aux3_imp_time_acc_2:
+  "t \<noteq> 0 \<Longrightarrow> (IMP_Minus_State_To_IMP_Minus_Minus_partial_tail_aux3_imp_time t s) = t + (IMP_Minus_State_To_IMP_Minus_Minus_partial_tail_aux3_imp_time 0 s)"
+  by (rule IMP_Minus_State_To_IMP_Minus_Minus_partial_tail_aux3_imp_time_acc_2_aux)            
+
+lemma IMP_Minus_State_To_IMP_Minus_Minus_partial_tail_aux3_imp_time_acc_3:
+  "(IMP_Minus_State_To_IMP_Minus_Minus_partial_tail_aux3_imp_time (a + b) s) = a + (IMP_Minus_State_To_IMP_Minus_Minus_partial_tail_aux3_imp_time b s)"
+  by (induction a arbitrary: b s) (simp add: IMP_Minus_State_To_IMP_Minus_Minus_partial_tail_aux3_imp_time_acc)+  
+
+abbreviation "IMP_Minus_State_To_IMP_Minus_Minus_partial_tail_aux3_AND_neq_zero_result \<equiv> ''AND_neq_zero_result''"
+abbreviation "IMP_Minus_State_To_IMP_Minus_Minus_partial_tail_aux3_LESS_neq_zero_result \<equiv> ''LESS_neq_zero_result''"
+
+abbreviation "IMP_Minus_State_To_IMP_Minus_Minus_partial_tail_aux3_IMP_if1 \<equiv>
+  \<comment> \<open>  IMP_Minus_State_To_IMP_Minus_Minus_partial_tail_aux3_ret' = 1;\<close>
+  (IMP_Minus_State_To_IMP_Minus_Minus_partial_tail_aux3_ret_str) ::= (A (N 1))
+"
+
+abbreviation "IMP_Minus_State_To_IMP_Minus_Minus_partial_tail_aux3_IMP_else1 \<equiv>
+  \<comment> \<open>  IMP_Minus_State_To_IMP_Minus_Minus_partial_tail_aux3_ret' = 0;\<close>
+  (IMP_Minus_State_To_IMP_Minus_Minus_partial_tail_aux3_ret_str) ::= (A (N 0))
+"
+
+abbreviation "IMP_Minus_State_To_IMP_Minus_Minus_partial_tail_aux3_IMP_if2 \<equiv>
+  \<comment> \<open>  LESS_neq_zero_a' = IMP_Minus_State_To_IMP_Minus_Minus_partial_tail_aux3_ko s;\<close>
+  (LESS_neq_zero_prefix @ LESS_neq_zero_a_str) ::= (A (V IMP_Minus_State_To_IMP_Minus_Minus_partial_tail_aux3_ko_str));;
+  \<comment> \<open>  LESS_neq_zero_b' = IMP_Minus_State_To_IMP_Minus_Minus_partial_tail_aux3_n s;\<close>
+  (LESS_neq_zero_prefix @ LESS_neq_zero_b_str) ::= (A (V IMP_Minus_State_To_IMP_Minus_Minus_partial_tail_aux3_n_str));;
+  \<comment> \<open>  LESS_neq_zero_ret' = 0;\<close>
+  (LESS_neq_zero_prefix @ LESS_neq_zero_ret_str) ::= (A (N 0));;
+  \<comment> \<open>  LESS_neq_zero_state = \<lparr>LESS_neq_zero_a = LESS_neq_zero_a',\<close>
+  \<comment> \<open>                         LESS_neq_zero_b = LESS_neq_zero_b',\<close>
+  \<comment> \<open>                         LESS_neq_zero_ret = LESS_neq_zero_ret'\<rparr>;\<close>
+  \<comment> \<open>  LESS_neq_zero_ret_state = LESS_neq_zero_imp LESS_neq_zero_state;\<close>
+  (invoke_subprogram LESS_neq_zero_prefix LESS_neq_zero_IMP_Minus);;
+  \<comment> \<open>  LESS_neq_zero_result = LESS_neq_zero_ret LESS_neq_zero_ret_state\<close>
+  (IMP_Minus_State_To_IMP_Minus_Minus_partial_tail_aux3_LESS_neq_zero_result) ::= (A (V (LESS_neq_zero_prefix @ LESS_neq_zero_ret_str)));;
+  \<comment> \<open>(if LESS_neq_zero_result \<noteq> 0 then\<close>
+  (IF IMP_Minus_State_To_IMP_Minus_Minus_partial_tail_aux3_LESS_neq_zero_result \<noteq>0 THEN
+    IMP_Minus_State_To_IMP_Minus_Minus_partial_tail_aux3_IMP_if1
+  \<comment> \<open>else\<close>
+  ELSE
+    IMP_Minus_State_To_IMP_Minus_Minus_partial_tail_aux3_IMP_else1
+  )
+"
+
+abbreviation "IMP_Minus_State_To_IMP_Minus_Minus_partial_tail_aux3_IMP_else2 \<equiv>
+  \<comment> \<open>  IMP_Minus_State_To_IMP_Minus_Minus_partial_tail_aux2_n' = IMP_Minus_State_To_IMP_Minus_Minus_partial_tail_aux3_n s;\<close>
+  (IMP_Minus_State_To_IMP_Minus_Minus_partial_tail_aux2_prefix @ IMP_Minus_State_To_IMP_Minus_Minus_partial_tail_aux2_n_str) ::=
+    (A (V IMP_Minus_State_To_IMP_Minus_Minus_partial_tail_aux3_n_str));;
+  \<comment> \<open>  IMP_Minus_State_To_IMP_Minus_Minus_partial_tail_aux2_v' = IMP_Minus_State_To_IMP_Minus_Minus_partial_tail_aux3_v s;\<close>
+  (IMP_Minus_State_To_IMP_Minus_Minus_partial_tail_aux2_prefix @ IMP_Minus_State_To_IMP_Minus_Minus_partial_tail_aux2_v_str) ::=
+    (A (V IMP_Minus_State_To_IMP_Minus_Minus_partial_tail_aux3_v_str));;
+  \<comment> \<open>  IMP_Minus_State_To_IMP_Minus_Minus_partial_tail_aux2_po' = IMP_Minus_State_To_IMP_Minus_Minus_partial_tail_aux3_po s;\<close>
+  (IMP_Minus_State_To_IMP_Minus_Minus_partial_tail_aux2_prefix @ IMP_Minus_State_To_IMP_Minus_Minus_partial_tail_aux2_po_str) ::=
+    (A (V IMP_Minus_State_To_IMP_Minus_Minus_partial_tail_aux3_po_str));;
+  \<comment> \<open>  IMP_Minus_State_To_IMP_Minus_Minus_partial_tail_aux2_vo' = IMP_Minus_State_To_IMP_Minus_Minus_partial_tail_aux3_vo s;\<close>
+  (IMP_Minus_State_To_IMP_Minus_Minus_partial_tail_aux2_prefix @ IMP_Minus_State_To_IMP_Minus_Minus_partial_tail_aux2_vo_str) ::=
+    (A (V IMP_Minus_State_To_IMP_Minus_Minus_partial_tail_aux3_vo_str));;
+  \<comment> \<open>  IMP_Minus_State_To_IMP_Minus_Minus_partial_tail_aux2_ko' = IMP_Minus_State_To_IMP_Minus_Minus_partial_tail_aux3_ko s;\<close>
+  (IMP_Minus_State_To_IMP_Minus_Minus_partial_tail_aux2_prefix @ IMP_Minus_State_To_IMP_Minus_Minus_partial_tail_aux2_ko_str) ::=
+    (A (V IMP_Minus_State_To_IMP_Minus_Minus_partial_tail_aux3_ko_str));;
+  \<comment> \<open>  IMP_Minus_State_To_IMP_Minus_Minus_partial_tail_aux2_ret' = 0;\<close>
+  (IMP_Minus_State_To_IMP_Minus_Minus_partial_tail_aux2_prefix @ IMP_Minus_State_To_IMP_Minus_Minus_partial_tail_aux2_ret_str) ::= (A (N 0));;
+  \<comment> \<open>  IMP_Minus_State_To_IMP_Minus_Minus_partial_tail_aux2_state =\<close>
+  \<comment> \<open>   \<lparr>IMP_Minus_State_To_IMP_Minus_Minus_partial_tail_aux2_n = IMP_Minus_State_To_IMP_Minus_Minus_partial_tail_aux2_n',\<close>
+  \<comment> \<open>    IMP_Minus_State_To_IMP_Minus_Minus_partial_tail_aux2_v = IMP_Minus_State_To_IMP_Minus_Minus_partial_tail_aux2_v',\<close>
+  \<comment> \<open>    IMP_Minus_State_To_IMP_Minus_Minus_partial_tail_aux2_po = IMP_Minus_State_To_IMP_Minus_Minus_partial_tail_aux2_po',\<close>
+  \<comment> \<open>    IMP_Minus_State_To_IMP_Minus_Minus_partial_tail_aux2_vo = IMP_Minus_State_To_IMP_Minus_Minus_partial_tail_aux2_vo',\<close>
+  \<comment> \<open>    IMP_Minus_State_To_IMP_Minus_Minus_partial_tail_aux2_ko = IMP_Minus_State_To_IMP_Minus_Minus_partial_tail_aux2_ko',\<close>
+  \<comment> \<open>    IMP_Minus_State_To_IMP_Minus_Minus_partial_tail_aux2_ret = IMP_Minus_State_To_IMP_Minus_Minus_partial_tail_aux2_ret'\<rparr>;\<close>
+  \<comment> \<open>  IMP_Minus_State_To_IMP_Minus_Minus_partial_tail_aux2_ret_state =\<close>
+  \<comment> \<open>    IMP_Minus_State_To_IMP_Minus_Minus_partial_tail_aux2_imp IMP_Minus_State_To_IMP_Minus_Minus_partial_tail_aux2_state;\<close>
+  (invoke_subprogram IMP_Minus_State_To_IMP_Minus_Minus_partial_tail_aux2_prefix IMP_Minus_State_To_IMP_Minus_Minus_partial_tail_aux2_IMP_Minus);;
+  \<comment> \<open>  IMP_Minus_State_To_IMP_Minus_Minus_partial_tail_aux3_ret' = \<close>
+  \<comment> \<open>    IMP_Minus_State_To_IMP_Minus_Minus_partial_tail_aux2_ret IMP_Minus_State_To_IMP_Minus_Minus_partial_tail_aux2_ret_state;\<close>
+  (IMP_Minus_State_To_IMP_Minus_Minus_partial_tail_aux3_ret_str) ::=
+    (A (V (IMP_Minus_State_To_IMP_Minus_Minus_partial_tail_aux2_prefix @ IMP_Minus_State_To_IMP_Minus_Minus_partial_tail_aux2_ret_str)))
+  \<comment> \<open>  ret = \<lparr>IMP_Minus_State_To_IMP_Minus_Minus_partial_tail_aux3_n = IMP_Minus_State_To_IMP_Minus_Minus_partial_tail_aux3_n s,\<close>
+  \<comment> \<open>         IMP_Minus_State_To_IMP_Minus_Minus_partial_tail_aux3_v = IMP_Minus_State_To_IMP_Minus_Minus_partial_tail_aux3_v s,\<close>
+  \<comment> \<open>         IMP_Minus_State_To_IMP_Minus_Minus_partial_tail_aux3_po = IMP_Minus_State_To_IMP_Minus_Minus_partial_tail_aux3_po s,\<close>
+  \<comment> \<open>         IMP_Minus_State_To_IMP_Minus_Minus_partial_tail_aux3_vo = IMP_Minus_State_To_IMP_Minus_Minus_partial_tail_aux3_vo s,\<close>
+  \<comment> \<open>         IMP_Minus_State_To_IMP_Minus_Minus_partial_tail_aux3_ko = IMP_Minus_State_To_IMP_Minus_Minus_partial_tail_aux3_ko s,\<close>
+  \<comment> \<open>         IMP_Minus_State_To_IMP_Minus_Minus_partial_tail_aux3_ret = IMP_Minus_State_To_IMP_Minus_Minus_partial_tail_aux3_ret'\<rparr>\<close>
+"
+
+definition IMP_Minus_State_To_IMP_Minus_Minus_partial_tail_aux3_IMP_Minus where
+  "IMP_Minus_State_To_IMP_Minus_Minus_partial_tail_aux3_IMP_Minus \<equiv>
+  \<comment> \<open>  EQUAL_neq_zero_a' = IMP_Minus_State_To_IMP_Minus_Minus_partial_tail_aux3_vo s;\<close>
+  (EQUAL_neq_zero_prefix @ EQUAL_neq_zero_a_str) ::= (A (V IMP_Minus_State_To_IMP_Minus_Minus_partial_tail_aux3_vo_str));;
+  \<comment> \<open>  EQUAL_neq_zero_b' = a_encode_char_as_nat;\<close>
+  (EQUAL_neq_zero_prefix @ EQUAL_neq_zero_b_str) ::= (A (N a_encode_char_as_nat));;
+  \<comment> \<open>  EQUAL_neq_zero_ret' = 0;\<close>
+  (EQUAL_neq_zero_prefix @ EQUAL_neq_zero_ret_str) ::= (A (N 0));;
+  \<comment> \<open>  EQUAL_neq_zero_state = \<lparr>EQUAL_neq_zero_a = EQUAL_neq_zero_a',\<close>
+  \<comment> \<open>                          EQUAL_neq_zero_b = EQUAL_neq_zero_b',\<close>
+  \<comment> \<open>                          EQUAL_neq_zero_ret = EQUAL_neq_zero_ret'\<rparr>;\<close>
+  \<comment> \<open>  EQUAL_neq_zero_ret_state = EQUAL_neq_zero_imp EQUAL_neq_zero_state;\<close>
+  (invoke_subprogram EQUAL_neq_zero_prefix EQUAL_neq_zero_IMP_Minus);;
+  \<comment> \<open>  AND_neq_zero_a' = IMP_Minus_State_To_IMP_Minus_Minus_partial_tail_aux3_po s;\<close>
+  (AND_neq_zero_prefix @ AND_neq_zero_a_str) ::= (A (V IMP_Minus_State_To_IMP_Minus_Minus_partial_tail_aux3_po_str));;
+  \<comment> \<open>  AND_neq_zero_b' = EQUAL_neq_zero_ret EQUAL_neq_zero_ret_state;\<close>
+  (AND_neq_zero_prefix @ AND_neq_zero_b_str) ::= (A (V (EQUAL_neq_zero_prefix @ EQUAL_neq_zero_ret_str)));;
+  \<comment> \<open>  AND_neq_zero_ret' = 0;\<close>
+  (AND_neq_zero_prefix @ AND_neq_zero_ret_str) ::= (A (N 0));;
+  \<comment> \<open>  AND_neq_zero_state = \<lparr>AND_neq_zero_a = AND_neq_zero_a',\<close>
+  \<comment> \<open>                        AND_neq_zero_b = AND_neq_zero_b',\<close>
+  \<comment> \<open>                        AND_neq_zero_ret = AND_neq_zero_ret'\<rparr>;\<close>
+  \<comment> \<open>  AND_neq_zero_ret_state = AND_neq_zero_imp AND_neq_zero_state;\<close>
+  (invoke_subprogram AND_neq_zero_prefix AND_neq_zero_IMP_Minus);;
+  \<comment> \<open>  AND_neq_zero_result = AND_neq_zero_ret AND_neq_zero_ret_state\<close>
+  (IMP_Minus_State_To_IMP_Minus_Minus_partial_tail_aux3_AND_neq_zero_result) ::= (A (V (AND_neq_zero_prefix @ AND_neq_zero_ret_str)));;
+  \<comment> \<open>(if AND_neq_zero_result \<noteq> 0 then\<close>
+  (IF IMP_Minus_State_To_IMP_Minus_Minus_partial_tail_aux3_AND_neq_zero_result \<noteq>0 THEN
+    IMP_Minus_State_To_IMP_Minus_Minus_partial_tail_aux3_IMP_if2
+  \<comment> \<open>else\<close>
+  ELSE
+    IMP_Minus_State_To_IMP_Minus_Minus_partial_tail_aux3_IMP_else2
+  )
+"
+
+abbreviation "IMP_Minus_State_To_IMP_Minus_Minus_partial_tail_aux3_IMP_vars \<equiv>
+  {IMP_Minus_State_To_IMP_Minus_Minus_partial_tail_aux3_n_str, IMP_Minus_State_To_IMP_Minus_Minus_partial_tail_aux3_v_str,
+  IMP_Minus_State_To_IMP_Minus_Minus_partial_tail_aux3_po_str, IMP_Minus_State_To_IMP_Minus_Minus_partial_tail_aux3_vo_str,
+  IMP_Minus_State_To_IMP_Minus_Minus_partial_tail_aux3_ko_str, IMP_Minus_State_To_IMP_Minus_Minus_partial_tail_aux3_ret_str,
+  IMP_Minus_State_To_IMP_Minus_Minus_partial_tail_aux3_AND_neq_zero_result, 
+  IMP_Minus_State_To_IMP_Minus_Minus_partial_tail_aux3_LESS_neq_zero_result}"
+
+definition "IMP_Minus_State_To_IMP_Minus_Minus_partial_tail_aux3_imp_to_HOL_state p s =
+  \<lparr>IMP_Minus_State_To_IMP_Minus_Minus_partial_tail_aux3_n = (s (add_prefix p IMP_Minus_State_To_IMP_Minus_Minus_partial_tail_aux3_n_str)),
+   IMP_Minus_State_To_IMP_Minus_Minus_partial_tail_aux3_v = (s (add_prefix p IMP_Minus_State_To_IMP_Minus_Minus_partial_tail_aux3_v_str)),
+   IMP_Minus_State_To_IMP_Minus_Minus_partial_tail_aux3_po = (s (add_prefix p IMP_Minus_State_To_IMP_Minus_Minus_partial_tail_aux3_po_str)),
+   IMP_Minus_State_To_IMP_Minus_Minus_partial_tail_aux3_vo = (s (add_prefix p IMP_Minus_State_To_IMP_Minus_Minus_partial_tail_aux3_vo_str)),
+   IMP_Minus_State_To_IMP_Minus_Minus_partial_tail_aux3_ko = (s (add_prefix p IMP_Minus_State_To_IMP_Minus_Minus_partial_tail_aux3_ko_str)),
+   IMP_Minus_State_To_IMP_Minus_Minus_partial_tail_aux3_ret = (s (add_prefix p IMP_Minus_State_To_IMP_Minus_Minus_partial_tail_aux3_ret_str))\<rparr>"
+
+lemmas IMP_Minus_State_To_IMP_Minus_Minus_partial_tail_aux3_state_translators =
+  IMP_Minus_State_To_IMP_Minus_Minus_partial_tail_aux3_imp_to_HOL_state_def
+  EQUAL_neq_zero_imp_to_HOL_state_def
+  AND_neq_zero_imp_to_HOL_state_def
+  LESS_neq_zero_imp_to_HOL_state_def
+  IMP_Minus_State_To_IMP_Minus_Minus_partial_tail_aux2_imp_to_HOL_state_def
+
+lemma IMP_Minus_State_To_IMP_Minus_Minus_partial_tail_aux3_IMP_Minus_correct_function:
+  "(invoke_subprogram p IMP_Minus_State_To_IMP_Minus_Minus_partial_tail_aux3_IMP_Minus, s) \<Rightarrow>\<^bsup>t\<^esup> s' \<Longrightarrow>
+     s' (add_prefix p IMP_Minus_State_To_IMP_Minus_Minus_partial_tail_aux3_ret_str)
+      = IMP_Minus_State_To_IMP_Minus_Minus_partial_tail_aux3_ret
+          (IMP_Minus_State_To_IMP_Minus_Minus_partial_tail_aux3_imp (IMP_Minus_State_To_IMP_Minus_Minus_partial_tail_aux3_imp_to_HOL_state p s))"
+  apply(subst IMP_Minus_State_To_IMP_Minus_Minus_partial_tail_aux3_imp.simps)
+  apply(simp only: IMP_Minus_State_To_IMP_Minus_Minus_partial_tail_aux3_IMP_Minus_def prefix_simps)
+  apply(erule Seq_E)+
+  apply(erule EQUAL_neq_zero_IMP_Minus_correct[where vars = "IMP_Minus_State_To_IMP_Minus_Minus_partial_tail_aux3_IMP_vars"])
+  subgoal premises p using p(10) by fastforce
+  apply(erule AND_neq_zero_IMP_Minus_correct[where vars = "IMP_Minus_State_To_IMP_Minus_Minus_partial_tail_aux3_IMP_vars"])
+  subgoal premises p using p(12) by fastforce
+  apply(erule If_E)
+  subgoal
+    apply(erule Seq_E)+
+    apply(erule LESS_neq_zero_IMP_Minus_correct[where vars = "IMP_Minus_State_To_IMP_Minus_Minus_partial_tail_aux3_IMP_vars"])
+    subgoal premises p using p(20) by fastforce
+    by(fastforce simp: IMP_Minus_State_To_IMP_Minus_Minus_partial_tail_aux3_state_translators
+      IMP_Minus_State_To_IMP_Minus_Minus_partial_tail_aux3_state_upd_def)
+  subgoal
+    apply(erule Seq_E)+
+    apply(erule IMP_Minus_State_To_IMP_Minus_Minus_partial_tail_aux2_IMP_Minus_correct[where vars = "IMP_Minus_State_To_IMP_Minus_Minus_partial_tail_aux3_IMP_vars"])
+    subgoal premises p using p(22) by fastforce
+    by(fastforce simp: IMP_Minus_State_To_IMP_Minus_Minus_partial_tail_aux3_state_translators
+      IMP_Minus_State_To_IMP_Minus_Minus_partial_tail_aux3_state_upd_def)     
+  done
+
+lemma IMP_Minus_State_To_IMP_Minus_Minus_partial_tail_aux3_IMP_Minus_correct_effects:
+  "\<lbrakk>(invoke_subprogram (p @ IMP_Minus_State_To_IMP_Minus_Minus_partial_tail_aux3_pref) IMP_Minus_State_To_IMP_Minus_Minus_partial_tail_aux3_IMP_Minus, s) \<Rightarrow>\<^bsup>t\<^esup> s';
+    v \<in> vars; \<not> (prefix IMP_Minus_State_To_IMP_Minus_Minus_partial_tail_aux3_pref v)\<rbrakk>
+   \<Longrightarrow> s (add_prefix p v) = s' (add_prefix p v)"
+  using com_add_prefix_valid'' com_only_vars prefix_def
+  by blast
+
+lemma IMP_Minus_State_To_IMP_Minus_Minus_partial_tail_aux3_IMP_Minus_correct_time:
+  "(invoke_subprogram p IMP_Minus_State_To_IMP_Minus_Minus_partial_tail_aux3_IMP_Minus, s) \<Rightarrow>\<^bsup>t\<^esup> s' \<Longrightarrow>
+     t = IMP_Minus_State_To_IMP_Minus_Minus_partial_tail_aux3_imp_time 0 (IMP_Minus_State_To_IMP_Minus_Minus_partial_tail_aux3_imp_to_HOL_state p s)"
+  apply(subst IMP_Minus_State_To_IMP_Minus_Minus_partial_tail_aux3_imp_time.simps)
+  apply(simp only: IMP_Minus_State_To_IMP_Minus_Minus_partial_tail_aux3_IMP_Minus_def prefix_simps)
+  apply(erule Seq_tE)+
+  apply(erule EQUAL_neq_zero_IMP_Minus_correct[where vars = "IMP_Minus_State_To_IMP_Minus_Minus_partial_tail_aux3_IMP_vars"])
+  subgoal premises p using p(19) by fastforce
+  apply(erule AND_neq_zero_IMP_Minus_correct[where vars = "IMP_Minus_State_To_IMP_Minus_Minus_partial_tail_aux3_IMP_vars"])
+  subgoal premises p using p(21) by fastforce
+  apply(erule If_tE)
+  subgoal
+    apply(erule Seq_tE)+
+    apply(erule LESS_neq_zero_IMP_Minus_correct[where vars = "IMP_Minus_State_To_IMP_Minus_Minus_partial_tail_aux3_IMP_vars"])
+    subgoal premises p using p(35) by fastforce
+    by(fastforce simp add: Let_def IMP_Minus_State_To_IMP_Minus_Minus_partial_tail_aux3_state_translators)  
+  subgoal
+    apply(erule Seq_tE)+
+    apply(erule IMP_Minus_State_To_IMP_Minus_Minus_partial_tail_aux2_IMP_Minus_correct[where vars = "IMP_Minus_State_To_IMP_Minus_Minus_partial_tail_aux3_IMP_vars"])
+    subgoal premises p using p(39) by fastforce
+    by(fastforce simp add: Let_def IMP_Minus_State_To_IMP_Minus_Minus_partial_tail_aux3_state_translators) 
+  done
+
+lemma IMP_Minus_State_To_IMP_Minus_Minus_partial_tail_aux3_IMP_Minus_correct:
+  "\<lbrakk>(invoke_subprogram (p1 @ p2) IMP_Minus_State_To_IMP_Minus_Minus_partial_tail_aux3_IMP_Minus, s) \<Rightarrow>\<^bsup>t\<^esup> s';
+    \<And>v. v \<in> vars \<Longrightarrow> \<not> (set p2 \<subseteq> set v);
+    \<lbrakk>t = (IMP_Minus_State_To_IMP_Minus_Minus_partial_tail_aux3_imp_time 0 (IMP_Minus_State_To_IMP_Minus_Minus_partial_tail_aux3_imp_to_HOL_state (p1 @ p2) s));
+     s' (add_prefix (p1 @ p2) IMP_Minus_State_To_IMP_Minus_Minus_partial_tail_aux3_ret_str) =
+          IMP_Minus_State_To_IMP_Minus_Minus_partial_tail_aux3_ret (IMP_Minus_State_To_IMP_Minus_Minus_partial_tail_aux3_imp
+                                        (IMP_Minus_State_To_IMP_Minus_Minus_partial_tail_aux3_imp_to_HOL_state (p1 @ p2) s));
+     \<And>v. v \<in> vars \<Longrightarrow> s (add_prefix p1 v) = s' (add_prefix p1 v)\<rbrakk>
+   \<Longrightarrow> P\<rbrakk> \<Longrightarrow> P"
+  using IMP_Minus_State_To_IMP_Minus_Minus_partial_tail_aux3_IMP_Minus_correct_function
+    IMP_Minus_State_To_IMP_Minus_Minus_partial_tail_aux3_IMP_Minus_correct_time
+    IMP_Minus_State_To_IMP_Minus_Minus_partial_tail_aux3_IMP_Minus_correct_effects
+  by (meson set_mono_prefix)
+
+(* ---------------------------------------------------------------------------------------------- *)
 
 fun IMP_Minus_State_To_IMP_Minus_Minus_partial_tail' :: "nat \<Rightarrow> nat \<Rightarrow> nat \<Rightarrow> nat \<Rightarrow> nat" where
   "IMP_Minus_State_To_IMP_Minus_Minus_partial_tail' s n r v =
